dataplane/Examples/Batch_op_Correctness.thy
@@ -61,12 +61,12 @@ abbreviation "l2 f \<equiv> Logic (batch_op (init_operator_state_ty2 default_int
 
 abbreviation "test_dt2 \<equiv> Comp [(0, 1) \<mapsto> (0, 1)] (l1 (\<lambda> _. inps2)) (l2 (\<lambda> b. if b = [] then trace (STR ''Empty batch! ! !'') [] else [Max (set b)]))"
 
-abbreviation "test_op2 \<equiv> compile_dataflow test_dt2 :: (2 \<times> 1, 2 \<times> 1, _) op"
+abbreviation "test_op \<equiv> compile_dataflow test_dt2 :: (2 \<times> 1, 2 \<times> 1, _) op"
 
-value [GHC] "lmap (\<lambda> io. case io of VOut p (x, t) \<Rightarrow> (projr x, t)) (trace_exec test_op2)"
-value [GHC] "check_prefix 100 [((1, 1), (Inr 10, MyPair 1 1)), ((1, 1), (Inr 7, MyPair 0 1)),((1, 1), (Inr 3, MyPair 1 0))] test_op2"
-value [GHC] "check_prefix 100 [((1, 1), (Inr 7, MyPair 0 1)), ((1, 1), (Inr 10, MyPair 1 1)), ((1, 1), (Inr 3, MyPair 1 0))] test_op2"
-value [GHC] "check_prefix 100 [((1, 1), (Inr 3, MyPair 1 0)), ((1, 1), (Inr 10, MyPair 1 1)), ((1, 1), (Inr 7, MyPair 0 1))] test_op2"
+value [GHC] "lmap (\<lambda> io. case io of VOut p (x, t) \<Rightarrow> (projr x, t)) (trace_exec test_op)"
+value [GHC] "check_prefix 100 [((1, 1), (Inr 10, MyPair 1 1)), ((1, 1), (Inr 7, MyPair 0 1)),((1, 1), (Inr 3, MyPair 1 0))] test_op"
+value [GHC] "check_prefix 100 [((1, 1), (Inr 7, MyPair 0 1)), ((1, 1), (Inr 10, MyPair 1 1)), ((1, 1), (Inr 3, MyPair 1 0))] test_op"
+value [GHC] "check_prefix 100 [((1, 1), (Inr 3, MyPair 1 0)), ((1, 1), (Inr 10, MyPair 1 1)), ((1, 1), (Inr 7, MyPair 0 1))] test_op"
 
 section \<open>Generalized Correctness\<close>
 
